nextSame Diff rework

Dafny/Common/SameDifferenece.i.dfy
@@ -64,6 +64,12 @@ module AbstractSameDifference {
         s.ok
     }
 
+    function impactedState() : (vars:set<name>) //specified 
+    {
+        var n:name := "x";
+        {n}
+    } 
+
     datatype Step =
         | updateStep(sv:stateVal) 
         | updateStepNonImpact(sv:stateVal) 
@@ -72,15 +78,20 @@ module AbstractSameDifference {
     predicate NextStep(s:state, s':state, step:Step)
     {
         match step  
-            case updateStep(sv) => sv.Val? && s' == updateVal(s,sv.n,sv.i) && s'.pc == s.pc+1
-            case updateStepNonImpact(sv) => sv.Val? && s' == updateVal(s,sv.n,sv.i) && s'.pc == s.pc+1
+            case updateStep(sv) => sv.Val? && s' == updateVal(s,sv) && s'.pc == s.pc+1
+            case updateStepNonImpact(sv) => sv.Val? &&  s' == updateVal(s,sv) && s'.pc == s.pc+1 // validNonImpactStep(sv) &&
             case stutterStep() => stutter(s,s')
+    }
+
+    predicate validNonImpactStep(sv:stateVal)
+    {
+        sv.Val? && !(sv.n in impactedState())
     }
 
     predicate StateNext(s:state,s':state)
     {
-        && exists step :: NextStep(s,s',step)
         && ValidState(s)
+        && exists step :: NextStep(s,s',step)
     
     }
 
@@ -103,55 +114,86 @@ module AbstractSameDifference {
             && forall i :: 0 <= i < |states|- 1 ==> StateNext(states[i],states[i+1]))
     }
 
-    function evalCode(c:simpleCode, s:state) : (b:behavior)
-        
-        decreases c, 0
-    {
-        // [s]
-        if |c| == 0 then    
-            []
-        else 
-            match first(c)
-                case Nil => [s] + evalCode(all_but_first(c),s)
-                case Val(n,i) =>  [updateVal(s,n,i)] + evalCode(all_but_first(c),updateVal(s,n,i))
-                case ValNonImpact(n,i) => [updateVal(s,n,i)] + evalCode(all_but_first(c),updateVal(s,n,i))
-    
-    }
-
-
-
-
-    function updateVal(s:state,n:name,val:int) : (s':state)
-        ensures s.ok ==> s'.ok
-    {
-        var s' := s.(vals := s.vals[n := val]);
-        s'
-    }
-
-    function ExecuteOneInst(s:state, s':state,step:Step) : (sv:stateVal)
+    lemma updateStepNonImpactImpliesSameImpactedState(s:state,s':state,step:Step)
+        requires StateNext(s,s')
         requires NextStep(s,s',step)
-        ensures !step.stutterStep? ==> step.sv == sv
-        // ensures step.updateStepNonImpact? ==> 
+        requires step.updateStepNonImpact?
+        requires !(step.sv.n in impactedState())
+        ensures !(step.sv.n in impactedState()) && (forall n :: n in s.vals && n != step.sv.n ==> s.vals[n] == s'.vals[n]);
+        ensures forall impact :: (impact in impactedState() && impact in s.vals) ==> s.vals[impact] == s'.vals[impact];
     {
-        // assume false;
-        if step.stutterStep? then
+        assert !(step.sv.n in impactedState()) && (forall n :: n in s.vals && n != step.sv.n ==> s.vals[n] == s'.vals[n]);
+        assert forall impact :: (impact in impactedState() && impact in s.vals) ==> s.vals[impact] == s'.vals[impact];
+    }
+
+
+    function updateVal(s:state,sv:stateVal) : (s':state)
+        requires sv.Val?
+        ensures s.ok ==> s'.ok
+        ensures if sv.n in s.vals && s.vals[sv.n] == sv.i then s.vals == s'.vals else s != s'
+        ensures s' == s.(vals := s.vals[sv.n := sv.i],pc := s.pc + 1)
+        ensures forall n :: n in s.vals && n != sv.n ==> s.vals[n] == s'.vals[n]
+    {
+        var s' := s.(vals := s.vals[sv.n := sv.i],pc := s.pc + 1);
+        assert s'.vals[sv.n] == sv.i;
+        if(sv.n in s.vals && s.vals[sv.n] == sv.i) then
+            assert s.vals == s'.vals;
+            s'
+        else 
+            assert s != s';
+            s'
+    }
+
+
+    function ExecuteOneInst(s:state, s':state) : (sv_diff:stateVal)
+        requires StateNext(s,s')
+
+        ensures forall step ::  (&& NextStep(s,s',step) 
+                                && step.updateStepNonImpact? 
+                                && !(step.sv.n in impactedState())) ==>  
+                                                                      || sv_diff.Nil? 
+                                                                      || (!(sv_diff.n in impactedState()) && (forall n :: n in s.vals && n != step.sv.n ==> s.vals[n] == s'.vals[n]));
+
+    {
+        var step :| NextStep(s,s',step);
+        if (step.stutterStep?) then
             var sv := Nil;
             sv
         else
             assert (step.updateStep? || step.updateStepNonImpact?);
-            assert s != s';
-            var sv:stateVal :| sv.Val? && updateVal(s,sv.n,sv.i) == s';
-            assert sv.n == step.sv.n;
-            sv 
+            if s.vals != s'.vals then
+                if forall name :: name in s'.vals ==> name in s.vals then // update val
+                    assert exists name :: name in s'.vals && name in s.vals && s.vals[name] != s'.vals[name];
+                    var diffKey :| diffKey in s'.vals && diffKey in s.vals && s.vals[diffKey] != s'.vals[diffKey];
+                    var diffVal := s'.vals[diffKey] - s.vals[diffKey];
+                    assert s' == s.(vals := s.vals[diffKey := s.vals[diffKey]+diffVal], pc := s.pc+1);
+                    assert step.updateStepNonImpact? ==> s' == updateVal(s, Val(diffKey,s'.vals[diffKey]));
+                    // assert step.updateStepNonImpact? ==> validNonImpactStep(step.sv);
+                    assert step.updateStepNonImpact? && !(step.sv.n in impactedState())==>  !(diffKey in impactedState()) && (forall n :: n in s.vals && n != step.sv.n ==> s.vals[n] == s'.vals[n]);
+                    Val(diffKey,diffVal)
+                else
+                    assert exists name :: name in s'.vals && !(name in s.vals);  
+                    var diffKey :|  diffKey in s'.vals && !(diffKey in s.vals);
+                    var diffVal := s'.vals[diffKey];
+                    assert s' == s.(vals := s.vals[diffKey := diffVal], pc := s.pc+1);
+                    Val(diffKey,diffVal)
+            else
+                Nil // no difference 
     }
 
-    predicate NextSameDiff(s:state, s':state, p:state, p':state, step:Step)
+    predicate NextSameDiff(s:state, s':state, p:state, p':state)
     {
-        && NextStep(s,s',step)
-        && NextStep(p,p',step)
+        && StateNext(s,s')
+        && StateNext(p,p')
         && s.pc == p.pc       
-        && ExecuteOneInst(s, s',step) == ExecuteOneInst(p, p',step)
+        && ExecuteOneInst(s, s') == ExecuteOneInst(p, p')
     }
+
+        s(x = 5, a = 1)  ,, p(x = 7, a = 900)
+        impactedSet = {x}
+        NonImpactStateTrans(add (a,5))
+        1 -> 6 ::  900 -> 905
+        s / s' == p / p'    
 
     lemma updateStepNonImpactImpliesNextSameDiff(s:state,p:state, nonDepenStep:Step)
         requires s.pc == p.pc  
@@ -160,58 +202,75 @@ module AbstractSameDifference {
         requires nonDepenStep.updateStepNonImpact?
         requires nonDepenStep.sv.Val?
         
-        ensures forall s',p' :: (NextStep(s,s',nonDepenStep) &&  NextStep(p,p',nonDepenStep)) ==> NextSameDiff(s,s',p,p',nonDepenStep);
+        // ensures forall s',p' :: (NextStep(s,s',nonDepenStep) &&  NextStep(p,p',nonDepenStep)) ==> NextSameDiff(s,s',p,p');
     {
 
-        forall s',p' | && s' == updateVal(s,nonDepenStep.sv.n,nonDepenStep.sv.i) 
-                       && p' == updateVal(p,nonDepenStep.sv.n,nonDepenStep.sv.i)
+        forall s',p' | && s' == updateVal(s,nonDepenStep.sv) 
+                       && p' == updateVal(p,nonDepenStep.sv)
                        && s'.pc == s.pc + 1
                        && p'.pc == p.pc + 1
-        ensures ExecuteOneInst(s, s',nonDepenStep) == ExecuteOneInst(p, p',nonDepenStep);
-        ensures NextSameDiff(s,s',p,p',nonDepenStep);
+        // ensures ExecuteOneInst(s, s') == ExecuteOneInst(p, p');
+        // ensures NextSameDiff(s,s',p,p');
         {
             
-             assert nonDepenStep.updateStepNonImpact?;
-             assert ExecuteOneInst(s,s',nonDepenStep).Val?;
-             assert ExecuteOneInst(s, s',nonDepenStep) == ExecuteOneInst(p, p',nonDepenStep);
-             assert NextSameDiff(s,s',p,p',nonDepenStep);
+            //  assert nonDepenStep.updateStepNonImpact?;
+            //  assert ExecuteOneInst(s,s').Val?;
+            //  assert ExecuteOneInst(s, s') == ExecuteOneInst(p, p');
+            //  assert NextSameDiff(s,s',p,p');
         }
 
     }
 
     
 
-    lemma subSeqOfBehaviorNextSameDiffIsBenign(b_s:behavior,subB_s:behavior,b_p:behavior,subB_p:behavior)
-        requires isSubSeq(b_s,subB_s)
-        requires ValidBehavior(b_s)
-        requires ValidBehavior(subB_s)
+    // lemma subSeqOfBehaviorNextSameDiffIsBenign(b_s:behavior,subB_s:behavior,b_p:behavior,subB_p:behavior)
+    //     requires isSubSeq(b_s,subB_s)
+    //     requires ValidBehavior(b_s)
+    //     requires ValidBehavior(subB_s)
 
-        requires isSubSeq(b_p,subB_p)
-        requires ValidBehavior(b_p)
-        requires ValidBehavior(subB_p)
+    //     requires isSubSeq(b_p,subB_p)
+    //     requires ValidBehavior(b_p)
+    //     requires ValidBehavior(subB_p)
 
-        requires |subB_s| == |subB_p|
-        requires |subB_s| > 0;
-        requires |b_p| >= (FindIndexInSeq(b_p,first(subB_p)) + |subB_p|-1)
-        requires forall i,step_s,step_p :: && (0 <= i < |subB_p|- 1) 
-                                           && NextStep(subB_s[i], subB_s[i+1], step_s)
-                                           && NextStep(subB_p[i], subB_p[i+1], step_p)  ==> step_s == step_p
+    //     requires |subB_s| == |subB_p|
+    //     requires |subB_s| > 0;
+    //     requires |b_p| >= (FindIndexInSeq(b_p,first(subB_p)) + |subB_p|-1)
+    //     requires forall i,step_s,step_p :: && (0 <= i < |subB_p|- 1) 
+    //                                        && NextStep(subB_s[i], subB_s[i+1], step_s)
+    //                                        && NextStep(subB_p[i], subB_p[i+1], step_p)  ==> step_s == step_p
                                      
-        requires forall i,step :: && (0 <= i < |subB_p|- 1) 
-                                  && NextStep(subB_s[i], subB_s[i+1], step)
-                                  && NextStep(subB_p[i], subB_p[i+1], step)  ==> step.updateStepNonImpact?
-    {
+    //     requires forall i,step :: && (0 <= i < |subB_p|- 1) 
+    //                               && NextStep(subB_s[i], subB_s[i+1], step)
+    //                               && NextStep(subB_p[i], subB_p[i+1], step)  ==> step.updateStepNonImpact?
+    // {
 
-        var first_index := FindIndexInSeq(b_p,first(subB_p));
-        assume (|b_p| >= (first_index + (|subB_p|-1)));
+    //     var first_index := FindIndexInSeq(b_p,first(subB_p));
+    //     assume (|b_p| >= (first_index + (|subB_p|-1)));
 
-        // assume IsBenign(b_p[first_index..first_index+|subB_p|]);
-    }
+    //     // assume IsBenign(b_p[first_index..first_index+|subB_p|]);
+    // }
 
     lemma patchIsBenign(c:simpleCode,patched:bool)
         // ensures forall s :: ValidState(s) ==> IsBenign(evalCode(c,s))
     {
 
     }
+
+
+    // function evalCode(c:simpleCode, s:state) : (b:behavior)
+        
+    //     decreases c, 0
+    // {
+    //     // [s]
+    //     if |c| == 0 then    
+    //         []
+    //     else 
+    //         match first(c)
+    //             case Nil => [s] + evalCode(all_but_first(c),s)
+    //             case Val(n,i) =>  [updateVal(s,n,i)] + evalCode(all_but_first(c),updateVal(s,n,i))
+    //             // case ValNonImpact(n,i) => [updateVal(s,n,i)] + evalCode(all_but_first(c),updateVal(s,n,i))
+    
+    // }
+
 
 }
