Dafny/examples/simpleBenign/simpleBenignisBenign.i.dfy
@@ -12,19 +12,28 @@ module simpleBenignIsBenign{
     import opened Collections__Seqs_s
 
 
-lemma unwrapMultiBehaviors(s:state) returns (b:behavior) 
+lemma unwrapMultiBehaviors(var_x:operand,s:state,patched:bool) returns (b:behavior) 
         requires ValidState(s);
         requires SOI_ASSIMPTIONS(s);
+        requires ValidOperand(s,var_x);
+        requires isInt(OperandContents(s,var_x))
+        requires OperandContents(s,var_x).itype.size == 4;
+        requires !OperandContents(s,var_x).itype.signed
+        requires OperandContents(s,var_x).val == 2 ==> patched
+
+        
         // ensures exists var_cmp2:operand :: var_cmp2.LV? && var_cmp2.l in s.lvs && var_cmp2.l == "var_cmp2";
-        ensures b == [s] + evalCodeRE(MergedTest(s),s);
+        ensures b == [s] + evalCodeRE(MergedTest(var_x,s,patched),s);
         // ensures ValidBehavior(b);
         // ensures forall r :: (ValidState(r) && SOI_ASSIMPTIONS(r) && s != r) ==> b == ([s] + evalCodeRE(benign_patch_SOI(r),r))
     {
         reveal_ValidBehavior();
-        var var_cmp2 := LV(" var_cmp2 ");
+         var var_cmp2 := LV(" var_cmp2 ");
+        var var_add := LV(" var_add ");
+        var var_z := LV(" var_z ");
         var var_0:operand :| var_0.LV? && var_0.l in s.lvs && var_0.l == "var_0";
     
-        var c := benign_patch_SOI(s);
+        var c := MergedTest(var_x,s,patched);
         // var if_end := Block([
         // Ins(ICMP(var_cmp2,ugt,4,var_0,D(Int(0,IntType(4,false))))),
         // IfElse(true,if_then3().block,if_end4().block)]);
@@ -33,9 +42,118 @@ lemma unwrapMultiBehaviors(s:state) returns (b:behavior)
         assert OperandContents(s,var_0).val >= 2147483646;
 
 
-        assert |c.block| == 2;
+        assert |c.block| == 3;
 
         b := [s] + evalCodeRE(c,s);
+        var step,remainder,subBehavior := unwrapBlockWitness(b,c.block,s);
+         assert b[0] == s;
+        // Ins(ADD(var_add,4,var_x,D(Int(2147483646,IntType(4,false)))))
+        assert (var_add.LV? || var_add.GV?);
+        assert ValidOperand(s,var_x);
+        assert ValidOperand(s,D(Int(2147483646,IntType(4,false))));
+        assert isInt(OperandContents(s,var_x));// && isInt(OperandContents(s,D(Int(2147483646,IntType(4,false)))));
+        //&& typesMatch(OperandContents(s,var_x),OperandContents(s,D(Int(2147483646,IntType(4,false)))));
+        assert ValidInstruction(s,ADD(var_add,4,var_x,D(Int(2147483646,IntType(4,false)))));
+        assert NextStep(b[0],b[1],Step.evalInsStep(ADD(var_add,4,var_x,D(Int(2147483646,IntType(4,false))))));
+        // assert OperandContents(b[0],var_0).val > 
+        assert StateNext(b[0],b[1]);
+        assert step == [b[1]];
+        assert remainder == [Divergence([Ins(ICMP(var_cmp2,sgt,4,var_add,D(Int(0,IntType(4,false)))))], [Ins(ICMP(var_cmp2,ugt,4,var_add,D(Int(0,IntType(4,false)))))],patched),
+        IfElse(var_cmp2,if_then3().block,if_end4().block)];
+        assert first(remainder).Divergence?;
+        assert subBehavior == b[1..];
+        assert subBehavior == [b[1]] + evalBlockRE(remainder, b[1]); // no state change, just control flow
+        assert b[2..] == evalBlockRE(remainder, b[1]);
+
+
+        var tempB := evalCodeRE(first(remainder),b[1]);
+        assert evalBlockRE(remainder, b[1]) == evalCodeRE(first(remainder),b[1]) + evalBlockRE(all_but_first(remainder),last(tempB));
+        if patched{
+
+        }else{
+            assert !patched ==> evalCodeRE(first(remainder),b[1]) == evalBlockRE(first(remainder).pre,b[1]);
+
+            assert subBehavior == [b[1]] + evalBlockRE(first(remainder).pre,b[1]) + evalBlockRE(all_but_first(remainder),last(tempB));
+
+            assert b[1] in subBehavior;
+            assert first(evalBlockRE(first(remainder).pre,b[1])) == b[2];
+            assert |first(remainder).pre| == 1;//Ins?;
+            assert first(remainder).pre[0].Ins?;
+            var oldRemainder := remainder;
+              //  assert evalBlockRE(first(remainder).pre,b[1]) == [evalInsRe(first(remainder).pre[0].ins,b[1])];
+        // assert forall c :: (c >= 0 && c < |evalBlockRE(first(remainder).pre,b[1])|) ==> evalBlockRE(first(remainder).pre,b[1])[c] == b[2+c];
+
+        // assert first(remainder) 
+        
+        step,remainder,subBehavior := unwrapBlockWitness(subBehavior,remainder,last(step));
+        assert step == [b[1]];//evalCodeRE(Divergence([Ins(ICMP(var_cmp2,sgt,4,var_add,D(Int(0,IntType(4,false)))))], [Ins(ICMP(var_cmp2,ugt,4,var_add,D(Int(0,IntType(4,false)))))],false),b[1]);
+                // step,remainder,subBehavior := unwrapBlockWitness(subBehavior,remainder,last(step));
+
+        // assert remainder == [Ins(ICMP(var_cmp2,sgt,4,var_add,D(Int(0,IntType(4,false)))))] + 
+        //                      [IfElse(var_cmp2,if_then3().block,if_end4().block)];
+        // // assert subBehavior == [b[1]] + evalBlockRE(remainder, b[1]); // no state change, just control flow
+        // //          assert all_but_first(oldRemainder) == all_but_first(remainder);
+        // //          tempB := evalCodeRE(first(remainder),b[1]);
+        // //          assert last(tempB) == b[1];
+        // //          assert first(oldRemainder).pre == [first(remainder)];
+        // //         //  assert evalBlockRE(first(oldRemainder).pre,b[1]) == evalBlockRE(first(remainder),b[1]) ;
+        // //          assert subBehavior == [b[1]] + evalCodeRE(first(remainder),b[1]) + evalBlockRE(all_but_first(remainder),last(tempB));
+
+        // // assert subBehavior == b[1..];
+        // // // assert first(b[1..]) == b[1];
+        // // assert first(remainder).Ins?;
+ 
+        // // assert all_but_first(remainder) == [IfElse(var_cmp2,if_then3().block,if_end4().block)];
+        // // assert first(remainder).ins == ICMP(var_cmp2,sgt,4,var_add,D(Int(0,IntType(4,false))));
+
+
+        // step,remainder,subBehavior := unwrapBlockWitness(subBehavior,remainder,last(step));
+
+        // assert ValidInstruction(b[1],ICMP(var_cmp2,sgt,4,var_add,D(Int(0,IntType(4,false)))));
+        // assert NextStep(b[1],b[2],Step.evalInsStep(ICMP(var_cmp2,sgt,4,var_add,D(Int(0,IntType(4,false))))));
+        // // assert OperandContents(b[0],var_0).val > 
+        // assert StateNext(b[1],b[2]);
+
+        // assert step == [b[2]];
+        // assert remainder == [IfElse(var_cmp2,if_then3().block,if_end4().block)];
+        // // // assert subBehavior == b[1..];
+        // // assert first(remainder).IfElse?;
+        // assert validIfCond(last(step),first(remainder).ifCond);
+        // // // assert dataToBool(OperandContents(last(step),first(remainder).ifCond));
+        // if dataToBool(OperandContents(last(step),first(remainder).ifCond)){ // True Branch
+        //     step,remainder,subBehavior := unwrapBlockWitness(subBehavior,remainder,last(step));
+
+        //     assert step == [b[2]];
+        //     assert remainder == if_then3().block;
+        //     assert subBehavior == [b[2]] + evalBlockRE(remainder, b[2]); // no state change, just control flow
+
+        //     assert first(remainder).Ins?;
+        //     assert first(remainder).ins == CALL(D(Void),printf_code(global_str()).block);
+        // //     // assert 
+        //     step,remainder,subBehavior := unwrapBlockWitness(subBehavior,remainder,last(step));
+        // //     assert |step| == 1;
+        //     // assert step == evalCodeRE(Ins(CALL(D(Void),printf_code(global_str()).block)),b[2]);
+        //     // assert step == [b[2]];
+        //     assert (step) == [evalInsRe(CALL(D(Void),printf_code(global_str()).block),b[2])];
+        //                 //  assert step == [b[3]];
+
+        // //     // unwrapPrintf(b[2],b[3],global_str());
+        // //     // assert NextStep(b[2],b[3],Step.evalInsStep(CALL(D(Void),printf_code(global_str()).block)));
+        // //     // assert StateNext(b[2],b[3]); 
+        // //     assert remainder == [if_end4()];
+        // //     assert first(remainder).Block?;
+        // //     // assert subBehavior == [b[3]] + evalBlockRE(remainder, b[3]);
+
+            
+        // //     step,remainder,subBehavior := unwrapBlockWitness(subBehavior,remainder,last(step));
+        // //     // assert step == [b[3]];
+        // //     assert remainder == if_end4().block;
+        // //     // assert subBehavior == [b[3]] + evalBlockRE(remainder, b[3]); // no state change, just control flow
+
+        // }
+        }
+        
+      
 
     }
 
@@ -57,6 +175,7 @@ lemma unwrapMultiBehaviors(s:state) returns (b:behavior)
         // IfElse(true,if_then3().block,if_end4().block)]);
 
         assert OperandContents(s,var_0).Int?;
+        assert OperandContents(s,var_0).itype.size == 4;
         assert OperandContents(s,var_0).val >= 2147483646;
 
 
@@ -215,6 +334,7 @@ lemma unwrapMultiBehaviors(s:state) returns (b:behavior)
             assert step == [b[1]];
             assert remainder == if_then3().block;
             assert subBehavior == [b[1]] + evalBlockRE(remainder, b[1]); // no state change, just control flow
+            // assert subBehavior == b[1..];
 
             assert first(remainder).Ins?;
             assert first(remainder).ins == CALL(D(Void),printf_code(global_str()).block);
